src/Std/Data/DTreeMap/Internal/WF/Lemmas.lean
@@ -1657,7 +1657,7 @@ theorem WF.constGetThenInsertIfNew?! {β : Type v} {_ : Ord α} [TransOrd α] {k
 ### `eraseMany!`
 -/
 
-theorem WF.eraseMany! {_ : Ord α} [TransOrd α] {ρ} [ForIn Id ρ α] {l : ρ}
+theorem WF.eraseMany! {_ : Ord α} [TransOrd α] {ρ} [ForIn Id ρ α] [ForInNew Id ρ α] {l : ρ}
     {t : Impl α β} (h : t.WF) : (t.eraseMany! l).1.WF :=
   (t.eraseMany! l).2 h (fun _ _ h' => h'.erase!)
 
@@ -1885,11 +1885,11 @@ theorem toListModel_insertMany!_list {_ : Ord α} [TransOrd α] [BEq α] [Lawful
     List.Perm (t.insertMany! l).val.toListModel (t.toListModel.insertList l) := by
   simpa only [← insertMany_eq_insertMany! h.balanced] using toListModel_insertMany_list h
 
-theorem WF.insertMany! {_ : Ord α} [TransOrd α] {ρ} [ForIn Id ρ ((a : α) × β a)] {l : ρ}
+theorem WF.insertMany! {_ : Ord α} [TransOrd α] {ρ} [ForIn Id ρ ((a : α) × β a)] [ForInNew Id ρ ((a : α) × β a)] {l : ρ}
     {t : Impl α β} (h : t.WF) : (t.insertMany! l).1.WF :=
   (t.insertMany! l).2 h (fun _ _ _ h' => h'.insert!)
 
-theorem WF.insertManyIfNew! {_ : Ord α} [TransOrd α] {ρ} [ForIn Id ρ ((a : α) × β a)] {l : ρ}
+theorem WF.insertManyIfNew! {_ : Ord α} [TransOrd α] {ρ} [ForIn Id ρ ((a : α) × β a)] [ForInNew Id ρ ((a : α) × β a)] {l : ρ}
     {t : Impl α β} (h : t.WF) : (t.insertManyIfNew! l).1.WF :=
   (t.insertManyIfNew! l).2 h (fun _ _ _ h' => h'.insertIfNew!)
 
@@ -1923,11 +1923,11 @@ theorem Const.beq_eq_beqModel {β : Type v} {_ : Ord α} [BEq α] [TransOrd α] 
   simp [beq, Const.beqModel, size_eq_length _ h₁.balanced, size_eq_length _ h₂.balanced, all_eq_all_toListModel,
     get?_eq_getValue? h₂.ordered]
 
-theorem WF.constInsertMany! {β : Type v} {_ : Ord α} [TransOrd α] {ρ} [ForIn Id ρ (α × β)] {l : ρ}
+theorem WF.constInsertMany! {β : Type v} {_ : Ord α} [TransOrd α] {ρ} [ForIn Id ρ (α × β)] [ForInNew Id ρ (α × β)]{l : ρ}
     {t : Impl α β} (h : t.WF) : (Const.insertMany! t l).1.WF :=
   (Const.insertMany! t l).2 h (fun _ _ _ h' => h'.insert!)
 
-theorem WF.constInsertManyIfNewUnit! {_ : Ord α} [TransOrd α] {ρ} [ForIn Id ρ α] {l : ρ}
+theorem WF.constInsertManyIfNewUnit! {_ : Ord α} [TransOrd α] {ρ} [ForIn Id ρ α] [ForInNew Id ρ α] {l : ρ}
     {t : Impl α Unit} (h : t.WF) : (Const.insertManyIfNewUnit! t l).1.WF :=
   (Const.insertManyIfNewUnit! t l).2 h (fun _ _ h' => h'.insertIfNew!)
 
